coq

coq/era_subst.v
@@ -14,9 +14,11 @@ Inductive era_agree_subst :
   nil ; nil ⊢ σ ~ σ ⊣ nil ; nil
 | era_agree_subst_ty Γ1 Δ1 σ1 σ2 Γ2 Δ2 A s :
   Γ1 ; Δ1 ⊢ σ1 ~ σ2 ⊣ Γ2 ; Δ2 ->
+  Γ2 ⊢ A : Sort s ->
   (A.[σ1] :: Γ1) ; (A.[σ1] :{s} Δ1) ⊢ up σ1 ~ up σ2 ⊣ (A :: Γ2) ; (A :{s} Δ2)
-| era_agree_subst_n Γ1 Δ1 σ1 σ2 Γ2 Δ2 A :
+| era_agree_subst_n Γ1 Δ1 σ1 σ2 Γ2 Δ2 A s :
   Γ1 ; Δ1 ⊢ σ1 ~ σ2 ⊣ Γ2 ; Δ2 ->
+  Γ2 ⊢ A : Sort s ->
   (A.[σ1] :: Γ1) ; (_: Δ1) ⊢ up σ1 ~ up σ2 ⊣ (A :: Γ2) ; (_: Δ2)
 | era_agree_subst_wk0 Γ1 Δ1 σ1 σ2 Γ2 Δ2 n n' A :
   Γ1 ; Δ1 ⊢ σ1 ~ σ2 ⊣ Γ2 ; Δ2 ->
@@ -30,14 +32,14 @@ Inductive era_agree_subst :
   Γ1 ; Δ1 ⊢ n .: σ1 ~ n' .: σ2 ⊣ (A :: Γ2) ; (A :{s} Δ2)
 | era_agree_subst_conv0 Γ1 Δ1 σ1 σ2 Γ2 Δ2 A B s :
   A === B ->
-  Γ1 ⊢ B.[ren (+1)].[σ1] : @s ->
-  Γ2 ⊢ B : @s ->
+  Γ1 ⊢ B.[ren (+1)].[σ1] : Sort s ->
+  Γ2 ⊢ B : Sort s ->
   Γ1 ; Δ1 ⊢ σ1 ~ σ2 ⊣ (A :: Γ2) ; (_: Δ2) ->
   Γ1 ; Δ1 ⊢ σ1 ~ σ2 ⊣ (B :: Γ2) ; (_: Δ2)
 | era_agree_subst_conv1 Γ1 Δ1 σ1 σ2 Γ2 Δ2 A B s :
   A === B ->
-  Γ1 ⊢ B.[ren (+1)].[σ1] : @s ->
-  Γ2 ⊢ B : @s ->
+  Γ1 ⊢ B.[ren (+1)].[σ1] : Sort s ->
+  Γ2 ⊢ B : Sort s ->
   Γ1 ; Δ1 ⊢ σ1 ~ σ2 ⊣ (A :: Γ2) ; (A :{s} Δ2) ->
   Γ1 ; Δ1 ⊢ σ1 ~ σ2 ⊣ (B :: Γ2) ; (B :{s} Δ2)
 where "Γ1 ; Δ1 ⊢ σ1 ~ σ2 ⊣ Γ2 ; Δ2" := (era_agree_subst Γ1 Δ1 σ1 σ2 Γ2 Δ2).
@@ -46,22 +48,27 @@ Lemma era_agree_subst_key Γ1 Γ2 Δ1 Δ2 σ1 σ2 s :
   Γ1 ; Δ1 ⊢ σ1 ~ σ2 ⊣ Γ2 ; Δ2 -> Δ2 ▷ s -> Δ1 ▷ s.
 Proof with eauto using key.
   move=>agr. elim: agr s=>{Γ1 Γ2 Δ1 Δ2 σ1 σ2}...
-  { move=>Γ1 Δ1 σ1 σ2 Γ2 Δ2 A s agr ih r k. inv k... }
-  { move=>Γ1 Δ1 σ1 σ2 Γ2 Δ2 _ agr ih s k. inv k... }
+  { move=>Γ1 Δ1 σ1 σ2 Γ2 Δ2 A s agr ih tyA r k. inv k... }
+  { move=>Γ1 Δ1 σ1 σ2 Γ2 Δ2 A s agr ih tyA r k. inv k... }
   { move=>Γ1 Δ1 σ1 σ2 Γ2 Δ2 n n' A agr ih tyn s k. inv k... }
   { move=>Γ1 Γ2 σ1 σ2 Δ1 Δ2 Δa Δb n n' A s k1 mrg agr ih tyn r k2.
     inv k2... apply: key_merge... apply: key_impure. }
   { move=>Γ1 Δ1 σ1 σ2 Γ2 Δ2 A B s eq tyB1 tyB2 agr ih r k. inv k... }
 Qed.
 
+Lemma era_dyn_agree_subst Γ1 Γ2 Δ1 Δ2 σ1 σ2 :
+  Γ1 ; Δ1 ⊢ σ1 ~ σ2 ⊣ Γ2 ; Δ2 -> Γ1 ; Δ1 ⊢ σ1 ⊣ Γ2 ; Δ2.
+Proof with eauto using dyn_agree_subst.
+  elim=>{Γ1 Γ2 Δ1 Δ2 σ1 σ2}...
+  move=>Γ1 Γ2 σ1 σ2 Δ1 Δ2 Δa Δb n n' A s k mrg agr ih tyn.
+  apply: dyn_agree_subst_wk1...
+  apply: era_dyn_type...
+Qed.
+
 Lemma era_sta_agree_subst Γ1 Γ2 Δ1 Δ2 σ1 σ2 :
   Γ1 ; Δ1 ⊢ σ1 ~ σ2 ⊣ Γ2 ; Δ2 -> Γ1 ⊢ σ1 ⊣ Γ2.
 Proof with eauto using sta_agree_subst.
-  elim=>{Γ1 Γ2 Δ1 Δ2 σ1 σ2}...
-  move=>Γ1 Γ2 σ1 σ2 Δ1 Δ2 Δa Δb n n' A s _ _ _ agr tyn.
-  constructor...
-  apply: dyn_sta_type...
-  apply: era_dyn_type...
+  move/era_dyn_agree_subst/dyn_sta_agree_subst=>//.
 Qed.
 
 Lemma era_agree_subst_refl Γ Δ : dyn_wf Γ Δ -> Γ ; Δ ⊢ ids ~ ids ⊣ Γ ; Δ.
@@ -80,31 +87,31 @@ Qed.
 Hint Resolve era_agree_subst_refl.
 
 Lemma era_agree_subst_has Γ1 Γ2 σ1 σ2 Δ1 Δ2 x A :
-  dyn_wf Γ1 Δ1 -> Γ1 ; Δ1 ⊢ σ1 ~ σ2 ⊣ Γ2 ; Δ2 -> dyn_has Δ2 x A ->
+  Γ1 ; Δ1 ⊢ σ1 ~ σ2 ⊣ Γ2 ; Δ2 -> dyn_wf Γ1 Δ1 -> dyn_has Δ2 x A ->
   Γ1 ; Δ1 ⊢ (σ1 x) ~ (σ2 x) : A.[σ1].
 Proof with eauto using era_agree_subst, era_agree_subst_key.
-  move=>wf agr. elim: agr wf x A=>{Γ1 Γ2 σ1 σ2 Δ1 Δ2}...
-  { move=>σ _ x A hs. inv hs. }
-  { move=>Γ1 Δ1 σ1 σ2 Γ2 Δ2 A s agr ih wf x B hs.
+  move=>agr. elim: agr x A=>{Γ1 Γ2 σ1 σ2 Δ1 Δ2}...
+  { move=>σ x A wf hs. inv hs. }
+  { move=>Γ1 Δ1 σ1 σ2 Γ2 Δ2 A s agr ih tyA x B wf hs.
     inv wf. inv hs; asimpl.
     replace A.[σ1 >> ren (+1)] with A.[σ1].[ren (+1)] by autosubst.
     apply: era_var; constructor...
     replace A0.[σ1 >> ren (+1)] with A0.[σ1].[ren (+1)] by autosubst.
     apply: era_eweakenU... }
-  { move=>Γ1 Δ1 σ1 σ2 Γ2 Δ2 A agr ih wf x B hs.
+  { move=>Γ1 Δ1 σ1 σ2 Γ2 Δ2 A s agr ih tyA x B wf hs.
     inv wf. inv hs; asimpl...
     replace A0.[σ1 >> ren (+1)] with A0.[σ1].[ren (+1)]
       by autosubst.
     apply: era_eweakenN... }
-  { move=>Γ1 Δ1 σ1 σ2 Γ2 Δ2 n n' A agr ih tyn wf x B hs. inv hs; asimpl... }
-  { move=>Γ1 Γ2 σ1 σ2 Δ1 Δ2 Δa Δb n n' A s k mrg agr ih tyn wf x B hs.
+  { move=>Γ1 Δ1 σ1 σ2 Γ2 Δ2 n n' A agr ih tyn x B wf hs. inv hs; asimpl... }
+  { move=>Γ1 Γ2 σ1 σ2 Δ1 Δ2 Δa Δb n n' A s k mrg agr ih tyn x B wf hs.
     inv hs; asimpl.
     { have ka:=era_agree_subst_key agr H4.
       have->//:=merge_pureL mrg ka. }
     { have->:=merge_pureR mrg k.
       apply: ih...
-      have[]//:=dyn_wf_merge mrg wf. } }
-  { move=>Γ1 Δ1 σ1 σ2 Γ2 Δ2 A B s eq tyB1 tyB2 agr ih wf x C hs. inv hs.
+      have[]//:=dyn_wf_inv mrg wf. } }
+  { move=>Γ1 Δ1 σ1 σ2 Γ2 Δ2 A B s eq tyB1 tyB2 agr ih x C wf hs. inv hs.
     { apply: era_conv.
       apply: sta_conv_subst.
       apply: sta_conv_subst...
@@ -124,14 +131,14 @@ Proof with eauto 6 using merge, era_agree_subst, era_agree_subst_key.
   move=>agr. elim: agr Δa Δb=>{Γ1 Γ2 Δ1 Δ2 σ1 σ2}.
   { move=>σ Δa Δb mrg. inv mrg.
     exists nil. exists nil... }
-  { move=>Γ1 Δ1 σ1 σ2 Γ2 Δ2 A s agr ih Δa Δb mrg. inv mrg.
+  { move=>Γ1 Δ1 σ1 σ2 Γ2 Δ2 A s agr ih tyA Δa Δb mrg. inv mrg.
     { have[Δa[Δb[mrg[agra agrb]]]]:=ih _ _ H2.
       exists (A.[σ1] :U Δa). exists (A.[σ1] :U Δb)... }
     { have[Δa[Δb[mrg[agra agrb]]]]:=ih _ _ H2.
       exists (A.[σ1] :L Δa). exists (_: Δb)... }
     { have[Δa[Δb[mrg[agra agrb]]]]:=ih _ _ H2.
       exists (_: Δa). exists (A.[σ1] :L Δb)... } }
-  { move=>Γ1 Δ1 σ1 σ2 Γ2 Δ2 A agr ih Δa Δb mrg. inv mrg.
+  { move=>Γ1 Δ1 σ1 σ2 Γ2 Δ2 A s agr ih tyA Δa Δb mrg. inv mrg.
     have[Δa[Δb[mrg[agra agrb]]]]:=ih _ _ H2.
     exists (_: Δa). exists (_: Δb)... }
   { move=>Γ1 Δ1 σ1 σ2 Γ2 Δ2 n n' A agr ih tyn Δa Δb mrg. inv mrg.
@@ -175,42 +182,33 @@ Proof with eauto 6 using merge, era_agree_subst, era_agree_subst_key.
 Qed.
 
 Lemma era_substitution Γ1 Γ2 m m' A Δ1 Δ2 σ1 σ2 :
-  dyn_wf Γ1 Δ1 -> Γ2 ; Δ2 ⊢ m ~ m' : A -> Γ1 ; Δ1 ⊢ σ1 ~ σ2 ⊣ Γ2 ; Δ2 ->
+  Γ2 ; Δ2 ⊢ m ~ m' : A -> Γ1 ; Δ1 ⊢ σ1 ~ σ2 ⊣ Γ2 ; Δ2 ->
   Γ1 ; Δ1 ⊢ m.[σ1] ~ m'.[σ2] : A.[σ1].
 Proof with eauto using era_agree_subst, era_agree_subst_key, era_type.
-  move=>wf ty. elim: ty Γ1 Δ1 σ1 σ2 wf=>{Γ2 Δ2 m m' A}.
-  { move=>Γ Δ x A shs dhs Γ1 Δ1 σ1 σ2 wf agr. asimpl.
-    apply: era_agree_subst_has... }
-  { move=>Γ Δ A B m m' s t k tyP tym ihm Γ1 Δ1 σ1 σ2 wf agr. asimpl.
-    have[r[tyA _]]:=sta_pi0_inv tyP.
-    apply: era_lam0...
-    have//:=sta_substitution tyP (era_sta_agree_subst agr).
-    apply: ihm...
-    apply: dyn_wf_n...
-    have:=sta_substitution tyA (era_sta_agree_subst agr).
-    asimpl... }
-  { move=>Γ Δ A B m m' s t k tyP tym ihm Γ1 Δ1 σ1 σ2 wf agr. asimpl.
-    have[r[tyA _]]:=sta_pi1_inv tyP.
-    apply: era_lam1...
-    have//:=sta_substitution tyP (era_sta_agree_subst agr).
-    apply: ihm...
-    apply: dyn_wf_ty...
-    have:=sta_substitution tyA (era_sta_agree_subst agr).
-    asimpl... }
-  { move=>Γ Δ A B m m' n s t tym ihm tyn Γ1 Δ1 σ1 σ2 wf agr. asimpl.
+  move=>ty. elim: ty Γ1 Δ1 σ1 σ2=>{Γ2 Δ2 m m' A}.
+  { move=>Γ Δ x A wf shs dhs Γ1 Δ1 σ1 σ2 agr. asimpl.
+    apply: era_agree_subst_has...
+    apply: dyn_substitution_wf...
+    apply: era_dyn_agree_subst... }
+  { move=>Γ Δ A B m m' s k tym ihm Γ1 Δ1 σ1 σ2 agr. asimpl.
+    have wf:=dyn_type_wf (era_dyn_type tym). inv wf.
+    apply: era_lam0... }
+  { move=>Γ Δ A B m m' s t k tym ihm Γ1 Δ1 σ1 σ2 agr. asimpl.
+    have wf:=dyn_type_wf (era_dyn_type tym). inv wf.
+    apply: era_lam1... }
+  { move=>Γ Δ A B m m' n s tym ihm tyn Γ1 Δ1 σ1 σ2 agr. asimpl.
     replace B.[n.[σ1] .: σ1] with B.[up σ1].[n.[σ1]/] by autosubst.
-    have{}ihm:=ihm _ _ _ _ wf agr.
+    have{}ihm:=ihm _ _ _ _ agr.
     apply: era_app0...
     have//:=sta_substitution tyn (era_sta_agree_subst agr). }
-  { move=>Γ Δ1 Δ2 Δ A B m m' n n' s t mrg tym ihm tyn ihn
-      Γ1 Δ0 σ1 σ2 wf agr. asimpl.
+  { move=>Γ Δ1 Δ2 Δ A B m m' n n' s mrg tym ihm tyn ihn
+      Γ1 Δ0 σ1 σ2 agr. asimpl.
     replace B.[n.[σ1] .: σ1] with B.[up σ1].[n.[σ1]/] by autosubst.
     have[Δa[Δb[mrg0[agra agrb]]]]:=era_agree_subst_merge agr mrg.
-    have[wfa wfb]:=dyn_wf_merge mrg0 wf.
-    have{}ihm:=ihm _ _ _ _ wfa agra.
-    have{}ihn:=ihn _ _ _ _ wfb agrb.
+    have{}ihm:=ihm _ _ _ _ agra.
+    have{}ihn:=ihn _ _ _ _ agrb.
     apply: era_app1... }
-  { move=>Γ Δ A B m m' s eq tym ihm tyB Γ1 Δ1 σ1 σ2 wf agr.
+  { move=>Γ Δ A B m m' s eq tym ihm tyB Γ1 Δ1 σ1 σ2 agr.
     apply: era_conv.
     apply: sta_conv_subst...
     apply: ihm...
@@ -219,24 +217,23 @@ Proof with eauto using era_agree_subst, era_agree_subst_key, era_type.
 Qed.
 
 Lemma era_subst0 Γ Δ m m' n A B :
-  dyn_wf Γ Δ -> (A :: Γ) ; _: Δ ⊢ m ~ m' : B -> Γ ⊢ n : A ->
-  Γ ; Δ ⊢ m.[n/] ~ m'.[Box/] : B.[n/].
+  (A :: Γ) ; _: Δ ⊢ m ~ m' : B -> Γ ⊢ n : A -> Γ ; Δ ⊢ m.[n/] ~ m'.[Box/] : B.[n/].
 Proof with eauto using era_agree_subst_refl.
-  move=>wf tym tyn.
+  move=>tym tyn.
+  have wf:=dyn_type_wf (era_dyn_type tym). inv wf.
   apply: era_substitution...
   apply: era_agree_subst_wk0...
   by asimpl.
 Qed.
 
 Lemma era_subst1 Γ Δ1 Δ2 Δ m m' n n' A B s :
-  dyn_wf Γ Δ -> Δ2 ▷ s -> Δ1 ∘ Δ2 => Δ ->
-  (A :: Γ) ; A :{s} Δ1 ⊢ m ~ m' : B -> Γ ; Δ2 ⊢ n ~ n' : A ->
-  Γ ; Δ ⊢ m.[n/] ~ m'.[n'/] : B.[n/].
+  Δ2 ▷ s -> Δ1 ∘ Δ2 => Δ ->
+  (A :: Γ) ; A :{s} Δ1 ⊢ m ~ m' : B -> Γ ; Δ2 ⊢ n ~ n' : A -> Γ ; Δ ⊢ m.[n/] ~ m'.[n'/] : B.[n/].
 Proof with eauto using era_agree_subst_refl.
-  move=>wf k mrg tym tyn.
+  move=>k mrg tym tyn.
+  have wf:=dyn_type_wf (era_dyn_type tym). inv wf.
   apply: era_substitution...
   apply: era_agree_subst_wk1...
-  have[wf1 wf2]:=dyn_wf_merge mrg wf...
   by asimpl.
 Qed.
 
@@ -244,7 +241,6 @@ Lemma era_esubst0 Γ Δ m m' n n' v A B B' :
   m' = m.[v/] ->
   n' = n.[Box/] ->
   B' = B.[v/] ->
-  dyn_wf Γ Δ ->
   (A :: Γ) ; _: Δ ⊢ m ~ n : B -> Γ ⊢ v : A ->
   Γ ; Δ ⊢ m' ~ n' : B'.
 Proof.
@@ -255,7 +251,7 @@ Lemma era_esubst1 Γ Δ1 Δ2 Δ m m' n n' v v' A B B' s :
   m' = m.[v/] ->
   n' = n.[v'/] ->
   B' = B.[v/] ->
-  dyn_wf Γ Δ -> Δ2 ▷ s -> Δ1 ∘ Δ2 => Δ ->
+  Δ2 ▷ s -> Δ1 ∘ Δ2 => Δ ->
   (A :: Γ) ; A :{s} Δ1 ⊢ m ~ n : B ->
   Γ ; Δ2 ⊢ v ~ v' : A ->
   Γ ; Δ ⊢ m' ~ n' : B'.
@@ -264,11 +260,11 @@ Proof.
 Qed.
 
 Lemma era_ctx_conv0 Γ Δ m m' A B C s :
-  dyn_wf (B :: Γ) (_: Δ) -> B === A ->
-  Γ ⊢ A : @s -> (A :: Γ) ; _: Δ ⊢ m ~ m' : C ->
-  (B :: Γ) ; _: Δ ⊢ m ~ m' : C.
-Proof with eauto.
-  move=>wf eq tyA tym.
+  B === A ->
+  Γ ⊢ B : Sort s -> (A :: Γ) ; _: Δ ⊢ m ~ m' : C -> (B :: Γ) ; _: Δ ⊢ m ~ m' : C.
+Proof with eauto using dyn_wf, era_agree_subst_refl.
+  move=>eq tyB tym.
+  have wf:=dyn_type_wf (era_dyn_type tym). inv wf.
   have:(B :: Γ) ; _: Δ ⊢ m.[ids] ~ m'.[ids] : C.[ids].
   apply: era_substitution...
   apply: era_agree_subst_conv0...
@@ -279,11 +275,11 @@ Proof with eauto.
 Qed.
 
 Lemma era_ctx_conv1 Γ Δ m m' A B C s :
-  dyn_wf (B :: Γ) (B :{s} Δ) -> B === A ->
-  Γ ⊢ A : @s -> (A :: Γ) ; A :{s} Δ ⊢ m ~ m' : C ->
-  (B :: Γ) ; B :{s} Δ ⊢ m ~ m' : C.
-Proof with eauto.
-  move=>wf eq tyA tym.
+  B === A ->
+  Γ ⊢ B : Sort s -> (A :: Γ) ; A :{s} Δ ⊢ m ~ m' : C -> (B :: Γ) ; B :{s} Δ ⊢ m ~ m' : C.
+Proof with eauto using dyn_wf, era_agree_subst_refl.
+  move=>eq tyA tym.
+  have wf:=dyn_type_wf (era_dyn_type tym). inv wf.
   have:(B :: Γ) ; B :{s} Δ ⊢ m.[ids] ~ m'.[ids] : C.[ids].
   apply: era_substitution...
   apply: era_agree_subst_conv1...
