coq/era_prog.v
@@ -6,19 +6,19 @@ Set Implicit Arguments.
 Unset Strict Implicit.
 Unset Printing Implicit Defensive.
 
-Lemma era_lam0_canonical Γ Δ A B m n s t :
-  Γ ; Δ ⊢ Lam0 A m s t ~ n : B -> exists m', n = Lam0 Box m' s t.
+Lemma era_lam0_canonical Γ Δ A B m n s :
+  Γ ; Δ ⊢ Lam0 A m s ~ n : B -> exists m', n = Lam0 Box m' s.
 Proof with eauto.
-  move e:(Lam0 A m s t)=>x ty. elim: ty A m s t e=>//{Γ Δ x n B}.
-  move=>Γ Δ A B m m' s t k tyP tym ihm A0 m0 s0 t0 [e1 e2 e3 e4]; subst.
+  move e:(Lam0 A m s)=>x ty. elim: ty A m s e=>//{Γ Δ x n B}.
+  move=>Γ Δ A B m m' s k tym ihm A0 m0 s0[e1 e2 e3]; subst.
   exists m'...
 Qed.
 
-Lemma era_lam1_canonical Γ Δ A B m n s t :
-  Γ ; Δ ⊢ Lam1 A m s t ~ n : B -> exists m', n = Lam1 Box m' s t.
+Lemma era_lam1_canonical Γ Δ A B m n s :
+  Γ ; Δ ⊢ Lam1 A m s ~ n : B -> exists m', n = Lam1 Box m' s.
 Proof with eauto.
-  move e:(Lam1 A m s t)=>x ty. elim: ty A m s t e=>//{Γ Δ x n B}.
-  move=>Γ Δ A B m m' s t k tyP tym ihm A0 m0 s0 t0 [e1 e2 e3 e4]; subst.
+  move e:(Lam1 A m s)=>x ty. elim: ty A m s e=>//{Γ Δ x n B}.
+  move=>Γ Δ A B m m' s t k tym ihm A0 m0 s0[e1 e2 e3]; subst.
   exists m'...
 Qed.
 
@@ -27,12 +27,12 @@ Lemma era_prog m m' A :
 Proof with eauto using dyn_step, dyn_val.
   move e1:(nil)=>Γ.
   move e2:(nil)=>Δ ty. elim: ty e1 e2=>{Γ Δ m m' A}.
-  { move=>Γ Δ x A shs dhs e1 e2; subst. inv shs. }
-  { move=>Γ Δ A B m m' s t k tyP tym ihm e1 e2; subst.
+  { move=>Γ Δ x A wf shs dhs e1 e2; subst. inv shs. }
+  { move=>Γ Δ A B m m' s k tym ihm e1 e2; subst.
     right... }
-  { move=>Γ Δ A B m m' s t k tyP tym ihm e1 e2; subst.
+  { move=>Γ Δ A B m m' s t k tym ihm e1 e2; subst.
     right... }
-  { move=>Γ Δ A B m m' n s t erm ihm tyn e1 e2; subst.
+  { move=>Γ Δ A B m m' n s erm ihm tyn e1 e2; subst.
     have[[x st]|vl]:=ihm erefl erefl.
     { left. exists (App x Box)... }
     { left.
@@ -41,7 +41,7 @@ Proof with eauto using dyn_step, dyn_val.
       have[A0[n0 e]]:=dyn_pi0_canonical tym (convR _ _) vl. subst.
       have[m0 e]:=era_lam0_canonical erm. subst.
       exists (m0.[Box/])... } }
-  { move=>Γ Δ1 Δ2 Δ A B m m' n n' s t mrg erm ihm ern ihn e1 e2; subst.
+  { move=>Γ Δ1 Δ2 Δ A B m m' n n' s mrg erm ihm ern ihn e1 e2; subst.
     inv mrg. have[[mx st1]|vlm]:=ihm erefl erefl.
     { left. exists (App mx n')... }
     { left. have[[nx st2]|vln]:=ihn erefl erefl.
