coq/era_type.v
@@ -9,32 +9,31 @@ Unset Printing Implicit Defensive.
 Reserved Notation "Γ ; Δ ⊢ m ~ n : A" (at level 50, Δ, m, n, A at next level).
 Inductive era_type : sta_ctx -> dyn_ctx -> term -> term -> term -> Prop :=
 | era_var Γ Δ x A :
+  dyn_wf Γ Δ ->
   sta_has Γ x A ->
   dyn_has Δ x A ->
   Γ ; Δ ⊢ Var x ~ Var x : A
-| era_lam0 Γ Δ A B m m' s t :
-  Δ ▷ t ->
-  Γ ⊢ Pi0 A B s t : @t ->
+| era_lam0 Γ Δ A B m m' s :
+  Δ ▷ s ->
   (A :: Γ) ; _: Δ ⊢ m ~ m' : B ->
-  Γ ; Δ ⊢ Lam0 A m s t ~ Lam0 Box m' s t : Pi0 A B s t
+  Γ ; Δ ⊢ Lam0 A m s ~ Lam0 Box m' s : Pi0 A B s
 | era_lam1 Γ Δ A B m m' s t :
-  Δ ▷ t ->
-  Γ ⊢ Pi1 A B s t : @t ->
-  (A :: Γ) ; A :{s} Δ ⊢ m ~ m' : B ->
-  Γ ; Δ ⊢ Lam1 A m s t ~ Lam1 Box m' s t : Pi1 A B s t
-| era_app0 Γ Δ A B m m' n s t :
-  Γ ; Δ ⊢ m ~ m' : Pi0 A B s t ->
+  Δ ▷ s ->
+  (A :: Γ) ; A :{t} Δ ⊢ m ~ m' : B ->
+  Γ ; Δ ⊢ Lam1 A m s ~ Lam1 Box m' s : Pi1 A B s
+| era_app0 Γ Δ A B m m' n s :
+  Γ ; Δ ⊢ m ~ m' : Pi0 A B s ->
   Γ ⊢ n : A ->
   Γ ; Δ ⊢ App m n ~ App m' Box : B.[n/]
-| era_app1 Γ Δ1 Δ2 Δ A B m m' n n' s t :
+| era_app1 Γ Δ1 Δ2 Δ A B m m' n n' s :
   Δ1 ∘ Δ2 => Δ ->
-  Γ ; Δ1 ⊢ m ~ m' : Pi1 A B s t ->
+  Γ ; Δ1 ⊢ m ~ m' : Pi1 A B s ->
   Γ ; Δ2 ⊢ n ~ n' : A ->
   Γ ; Δ ⊢ App m n ~ App m' n' : B.[n/]
 | era_conv Γ Δ A B m m' s :
   A === B ->
   Γ ; Δ ⊢ m ~ m' : A ->
-  Γ ⊢ B : @s ->
+  Γ ⊢ B : Sort s ->
   Γ ; Δ ⊢ m ~ m' : B
 where "Γ ; Δ ⊢ m ~ n : A" := (era_type Γ Δ m n A).
 
@@ -46,17 +45,17 @@ Lemma dyn_era_type Γ Δ m A :
   Γ ; Δ ⊢ m : A -> exists m', Γ ; Δ ⊢ m ~ m' : A.
 Proof with eauto using era_type.
   elim=>{Γ Δ m A}.
-  { move=>Γ Δ x A shs dhs. exists (Var x)... }
-  { move=>Γ Δ A B m s t k tyP tym [m' er].
-    exists (Lam0 Box m' s t)... }
-  { move=>Γ Δ A B m s t k tyP tym [m' er].
-    exists (Lam1 Box m' s t)... }
-  { move=>Γ Δ A B m n s t tym [m' er] tyn.
+  { move=>Γ Δ x A wf shs dhs. exists (Var x)... }
+  { move=>Γ Δ A B m s k tym[m' er].
+    exists (Lam0 Box m' s)... }
+  { move=>Γ Δ A B m s t k tym[m' er].
+    exists (Lam1 Box m' s)... }
+  { move=>Γ Δ A B m n s tym[m' er]tyn.
     exists (App m' Box).
     apply: era_app0... }
-  { move=>Γ Δ1 Δ2 Δ A B m n s t mrg tym [m' erm] tyn [n' ern].
+  { move=>Γ Δ1 Δ2 Δ A B m n s mrg tym[m' erm]tyn[n' ern].
     exists (App m' n').
     apply: era_app1... }
-  { move=>Γ Δ A B m s eq tym [m' er] tyB.
+  { move=>Γ Δ A B m s eq tym[m' er]tyB.
     exists m'. apply: era_conv... }
 Qed.
